high2/Zeta.High.Verifier.fst
@@ -1,10 +1,33 @@
 module Zeta.High.Verifier
 
+let contains_only_app_keys_comp (#app:_) (st: store_t app) (ks: S.seq base_key)
+  : b:bool { b <==> contains_only_app_keys st ks }
+  = admit()
+
+let puts (#app:_)
+  (vs: vtls_t app{vs.valid})
+  (ks: S.seq base_key)
+  (ws: S.seq (app_value_nullable app.adm))
+  : vs': vtls_t app{vs'.valid}
+  = admit()
+
 let lemma_high_verifier (aprm: app_params)
   : Lemma (ensures (GV.clock_monotonic_prop (high_verifier_spec_base aprm) /\
                     GV.thread_id_constant_prop (high_verifier_spec_base aprm) /\
                     GV.evict_prop (high_verifier_spec_base aprm) /\
                     GV.add_prop (high_verifier_spec_base aprm)))
+  = admit()
+
+let runapp_doesnot_change_nonref_slots
+  (#app: _)
+  (e: vlog_entry app {GV.RunApp? e})
+  (vs: vtls_t app)
+  (k: base_key)
+  : Lemma (requires (let GV.RunApp _ _ ks = e in
+                     let vs' = GV.verify_step e vs in
+                     vs'.valid /\ not (S.mem k ks)))
+          (ensures (let vs' = GV.verify_step e vs in
+                    vs.st k == vs'.st k))
   = admit()
 
 let runapp_doesnot_change_store_addmethod
@@ -17,4 +40,62 @@ let runapp_doesnot_change_store_addmethod
                     store_contains vs.st ki ==>
                     store_contains vs_post.st ki /\
                     add_method_of vs.st ki = add_method_of vs_post.st ki))
+  = admit()
+
+let runapp_implies_store_contains
+  (#app: _)
+  (e: vlog_entry app {GV.is_appfn e})
+  (vs: vtls_t _)
+  (k: base_key)
+  : Lemma (ensures (let GV.RunApp _ _ ks = e in
+                    let vs_post = GV.verify_step e vs in
+                    vs_post.valid ==>
+                    S.mem k ks ==>
+                    (let rs = GV.reads vs ks in
+                     let i = S.index_mem k ks in
+                     let ak,av = S.index rs i in
+                     store_contains vs.st k /\
+                     stored_key vs.st k = AppK ak /\
+                     stored_value vs.st k = AppV av)))
+  = admit()
+
+let runapp_doesnot_change_slot_emptiness
+  (#app: _)
+  (e: vlog_entry app {GV.is_appfn e})
+  (vs: vtls_t _)
+  (k: base_key)
+  : Lemma
+          (ensures (let vs_post = GV.verify_step e vs in
+                    vs_post.valid ==>
+                    ((store_contains vs.st k) <==> (store_contains vs_post.st k))))
+  = admit()
+
+let runapp_doesnot_change_slot_key
+  (#app:_)
+  (ki: base_key)
+  (e: vlog_entry app {Zeta.GenericVerifier.RunApp? e})
+  (vs: vtls_t app)
+  : Lemma (ensures (let vs_post = Zeta.GenericVerifier.verify_step e vs in
+                    vs_post.valid ==>
+                    store_contains vs.st ki ==>
+                    store_contains vs_post.st ki /\
+                    stored_key vs.st ki = stored_key vs_post.st ki))
+  = admit()
+
+let puts_valid
+  (#app:_)
+  (ki: base_key)
+  (e: vlog_entry app {GV.is_appfn e})
+  (vs: vtls_t app)
+  (i:nat)
+  : Lemma (ensures (let GV.RunApp f p ks = e in
+                    let vs_post = GV.verify_step e vs in
+                    vs_post.valid ==>
+                    i < S.length ks ==>
+                    (let rs = GV.reads vs ks in
+                     let fn = appfn f in
+                     let _,_,ws = fn p rs in
+                     let k = S.index ks i in
+                     store_contains vs_post.st k /\
+                     stored_value vs_post.st k = AppV (S.index ws i))))
   = admit()
